#### 1.3
a) $A = \{-3, -2, -1, 0, 1, 2\}$
b) $B = \emptyset$
c) $C = \{0, 1, 2, 3\}$
d) $D =  \{0, 3\}$
$y = {\mathbb{N}}$

#### 1.3
$(2^{2n + 1} - 2^{n + 1}  + 1)(2^{2n + 1} + 2^{n + 1}  + 1)$
$$
a = 2^{2n + 1} \quad b = 2^{n + 1}
$$

$$
\begin{align}
(a - b + 1)(a + b + 1) &= a^2 -b^2 + 2a + 1 \\
&= (2^{2n + 1})^2 - (2^{n + 1})^2 + 2*2^{2n+1} + 1 \\
&= 2^{2(2n + 1)} - 2^{2(n + 1)} +2^{2n + 2} + 1 \\
&= 2^{4n + 2} - 2^{2n + 2} + 2^{2n + 2} + 1\\
&= 2^{4n} *2^2 + 1 = 4 * 2^{4n} + 1 \\
&= 2^{4n + 2} + 1 = 2^{2(2n + 1)} + 1 \\
&= 4^{2n + 1} + 1
\end{align}
$$

#### 1.4



