## 13.2
$(i) \quad x\mapsto 5x^2 -6x + 2$
$x' \mapsto 10x -6$
Trouver tangente en $x_0 = 1$

$\lim\limits_{h \rightarrow 0} \frac{f(1 + h) -f(1)}{h} =\lim\limits_{x \rightarrow 0}\frac{5(h^2 + 2h + 1) -6-6h + 2 - 5 + 6 -2}{h}$

$\lim\limits_{x \rightarrow 0} \frac{5h^2 + 10h -6h}{h} = \lim\limits_{x \rightarrow 0} 5h + 4 = 4$



Calcule de la droite tangente
   $$
   y = t(x) = f(x_0) + f'(x_0)(x - x_0).
   $$

$y = f(1) + f'(1)(x-1) = 1 + 4(x-1) =4x-3$

Calcule de la droite normal
$$
   y = n(x) = f(x_0) - \frac{1}{f'(x_0)}(x - x_0).
$$
$y = f(1) - \frac{1}{f'(1)}(x-1) =1-\frac{1}{4}(x-1) = -\frac{1}{4}x + \frac{5}{4}$

tangente $= x' = 10x -6$
tangente: y = f(1) = 4 



## 13.4
$$
y = x^2 +px + q = f(x)
$$

$f'(x_0) = 2x_0 + p$

Donc
$f(1) = 2 + p + q = 1 \Rightarrow p + q = 0$
$f'(1) = 2 + p = 1 \Rightarrow p = -1$
$\Rightarrow q = 1$
$$
y = x^2 - x + 1
$$





