## 16.1

$(i)$ $f(x) = sin(2x + \frac{\pi}{5})$
$\quad f'(x) = cos(2x + \frac{\pi}{5}) \cdot 2$

$(ii) f(x) = cos(\sqrt{1-x^2})$

$f_1(x) = cos(x)$
$f_2(x) = \sqrt{x}$
$f_3(x) = 1-x^2$

$$
\begin{align}
f'(x) &= f_1'((f_2 \circ f_3)(x)) \cdot (f_2 \circ f_3)'(x) &=  f_1'((f_2 \circ f_3)(x)) \cdot f_2'(f_3(x)) \cdot f_3'(x) \\
&=-sin(\sqrt{1-x^2}) \cdot (\sqrt{1-x^2})'(x) &= -sin(\sqrt{1-x^2}) \cdot \frac{1}{2\sqrt{1-x^2}} \cdot -2x \\
\end{align}
$$
$= -x \cdot \frac{sin(\sqrt{1-x^2})}{\sqrt{1-x^2}}$

$(iii)$ $(cos(3x))'cos(5x) + cos(3x)(cos(5x))'$
$\quad = -3sin(3x)cos(5x) - 5cos(3x)(sin(5x))$

$(iv)$ $A sin(\omega x + \varphi),A,\omega > 0, \varphi\in\mathbb{R}$
$A \cdot cos(\omega x + \varphi) \cdot \omega$
