#### 5.1
![[Pasted image 20240927153714.png]]

i) $ln(\frac{18}{6} * 3^2) =ln(3^3) = 3ln(3)$
ii) $\frac{1}{2}log_{10}(2) + \frac{1}{2}log_{10}(4) = \frac{1}{2}log_{10}(8)$
iii) $\frac{e^3e^{2}}{e^{ln(3)}}e^{-\frac{3}{2}} =\frac{e^5}{3}\cdot e^{-\frac{3}{2}} =$


#### 5.2
$e^{4x} = 7 \Rightarrow ln(e^{4x}) = ln(7) \Rightarrow4x = ln(7) \Rightarrow x = \frac{ln(7)}{4}$
$log_{10}(x) +log_{10}(2x) = log_{10}(18) \Rightarrow log_{10}(2x^2) = log_{10}(18) \Rightarrow 2x^2 = 18 \Rightarrow x = 3$
iii) $log_2(x^2) \geq 8 \Leftrightarrow$
